cfrontend/BeePL_safety.v
@@ -157,12 +157,12 @@ match e with
 | Addr l ofs t => [::]
 | Eapp ef ts es t => flatten (map gen_safe_cond_expr es)
 | Hexpr h e t => [::] (* fix me *)
-| Screate _ _ _ => [::]
+| Screate _ _ _ _ => [::]
 | Sfield x a t => [::]
 | For e1 e2 d e t => [::]
 | Enone t => [::]
 | Esome e t => [::]
-| Match e pes t => [::]
+| Match e ps es t => [::]
 end.
 
 (* Defines the interpretation of safety condition *) 
